\documentclass{article}
\usepackage{epsfig}
\pagestyle{empty}
\begin{document}
$\mathbf{u}=\alpha $
\pagebreak

$\mathbf{u}=\alpha \mathbf{s}' \times (\mathbf{u}_\mathrm{n}-\mathbf{u}_\mathrm{s})+\alpha' \mathbf{s}' \times \left[ \mathbf{s}' \times (\mathbf{u}_\mathrm{n}-\b=\mathbf{u}_\mathrm{s})\right]$
\pagebreak

$\mathbf{u}=\alpha \mathbf{s}' \times (\mathbf{u}_\mathrm{n}-\mathbf{u}_\mathrm{s})$
\pagebreak

$\mathbf{u}=\alpha \mathbf{s}' \times (\mathbf{u}_\mathrm{n}-\mathbf{u}_\mathrm{s})+\alpha' \mathbf{s}' \times [\mathbf{s}' \times (\mathbf{u}_\mathrm{n}-\mathbf{u}_\mathrm{s})]$
\pagebreak

$\mathbf{u}=\alpha \mathbf{s}' \times (\mathbf{u}_\mathrm{n}-\mathbf{u}_\mathrm{s})+ \alpha' \mathbf{s}' \times [\mathbf{s}' \times (\mathbf{u}_\mathrm{n}-\mathbf{u}_\mathrm{s})]$
\pagebreak

$\mathbf{u}=\mathbf{u}_\mathrm{force}$
\pagebreak

\[ \frac{d \mathbf{s}_i}{d \xi}=\frac{\ell_{i-1}\mathbf{s}_{i+1}+(\ell_{i+1}-\ell_{i-1})\mathbf{s}_i+\ell_{i+1}\mathbf{s}_{i-1}} {2\ell_{i+1}\ell_{i-1}}+{\cal O}(\ell^2) \]
\pagebreak

\[ \frac{d^2 \mathbf{s}_i}{d \xi}^2=\frac{2\mathbf{s}_{i+1}}{\ell_{i+1}(\ell_{i+1}+\ell_{i- 1})}- \frac{2\mathbf{s}_i}{\ell_{i+1}\ell_{i-1}}+\frac{2\mathbf{s}_{i-1}}{\ell_{i-1}(\ell_{i+ 1}+\ell_{i-1})}+{\cal O}(\ell^2) \]
\pagebreak

\[ \frac{d^2 \mathbf{s}_i}{d \xi^2}=\frac{2\mathbf{s}_{i+1}}{\ell_{i+1}(\ell_{i+1}+\ell_{i- 1})}- \frac{2\mathbf{s}_i}{\ell_{i+1}\ell_{i-1}}+\frac{2\mathbf{s}_{i-1}}{\ell_{i-1}(\ell_{i+ 1}+\ell_{i-1})}+{\cal O}(\ell^2) \]
\pagebreak

$(x_1,y_1,z_1)$
\pagebreak

$(x_2,y_2,z_2)$
\pagebreak

$\sqrt{(x_2-x_1)^2+(y_2-y_1)^2+(z_2-z_1)^2}$
\pagebreak

${(x_2-x_1)^2+(y_2-y_1)^2+(z_2-z_1)^2}$
\pagebreak

$|\frac{d^2 \mathbf{s}_i}{d \xi^2}|$
\pagebreak

\[|\frac{d^2 \mathbf{s}_i}{d \xi^2}|\]
\pagebreak

$\mathbf{a}$
\pagebreak

$\mathbf{b}$
\pagebreak

\[ \theta=\cos^{-1} \mathbf{a} \cdot \mathbf{b} \]
\pagebreak

\[ \theta=\cos^{-1} \frac{ \mathbf{a} \cdot \mathbf{b}}{ab} \]
\pagebreak

$ \frac{d \mathbf{s}_i}{d \xi}=\frac{\mathbf{s}_{i+1}-\mathbf{s}_{i}}{\ell_i} $
\pagebreak

$\hat{\mathbf{s}''}$
\pagebreak

$\hat{\mathbf{s}'} \times \hat{\mathbf{s}''}$
\pagebreak

$\delta$
\pagebreak

\[ \mathbf{u}_n({\mathbf{x}},t)= \sum_{n=1}^{N_\textrm{KS}}\left(\mathbf{A}_n \times \mathbf{k}_n \cos\phi_n + {\bf B}_n \times \mathbf{k}_n \sin\phi_n \right), \]
\pagebreak

$\phi_n=\mathbf{k}_n \cdot \mathbf{x} + \omega_n t$\f, $
\pagebreak

$\mathbf{k}_n$\f and $
\pagebreak

$\phi_n=\mathbf{k}_n\cdot\mathbf{x}+\omega_n t$
\pagebreak

$N_\textrm{KS}$
\pagebreak

$\mathbf{k}_n$
\pagebreak

$\omega_n=k_n u_n$
\pagebreak

$\delta/2$
\pagebreak

$u=(B\cos(x),C\sin(y))$
\pagebreak

$u=(u_x,0,0)$
\pagebreak

$u=(0,0,u_0\exp{-z^2})$
\pagebreak

$u=(0,0,u_0\exp(-z^2))$
\pagebreak

$u=\nabla\phi$
\pagebreak

$\phi$
\pagebreak

\[ E=\frac{1}{2} \int_V \mathbf{u}^2 dV= =\Gamma \oint_{\cal L} \mathbf{u} \cdot \mathbf{r} \times \mathbf{s}' d\xi \]
\pagebreak

\[ \mathbf{s}_{i}^{n+1}=\mathbf{s}_{i}^{n}+\frac{\Delta t}{12}(23\mathbf{u}_{i}^{n} -16\mathbf{u}_{i}^{n-1}+5\mathbf{u}_{i}^{n-2})+\mathcal{O}(\Delta t^4) \]
\pagebreak

\[ x=y \]
\pagebreak

\[ E=\frac{1}{2} \int_V \mathbf{u}^2 dV= =\Gamma \oint_{\cal L} \mathbf{u} \cdot \mathbf{s} \times \mathbf{s}' d\xi \]
\pagebreak

\[ \frac{d\mathbf{s}_i}{dt}=\frac{\Gamma}{4\pi} \ln \left(\frac{\sqrt{\ell_i \ell_{i+1}}}{a}\right)\mathbf{s}_i' \times \mathbf{s}_i'' -\frac{\Gamma}{4 \pi} \oint_{\cal L'} \frac{(\mathbf{s}_i-\mathbf{r}) } {\vert \mathbf{s}_i - \mathbf{r} \vert^3} \times {\bf d}\mathbf{r} \]
\pagebreak

\[ \frac{d\mathbf{s}_i}{dt}=\frac{\Gamma}{4\pi} \ln \left(\frac{\sqrt{\ell_i \ell_{i+1}}}{a}\right)\mathbf{s}_i' \times \mathbf{s}_i'' +\frac{\Gamma}{4 \pi} \oint_{\cal L'} \frac{(\mathbf{s}_i-\mathbf{r}) } {\vert \mathbf{s}_i - \mathbf{r} \vert^3} \times {\bf d}\mathbf{r} \]
\pagebreak

\[\frac{\Gamma}{4 \pi} \oint_{\cal L} \frac{(\mathbf{s}_i-\mathbf{r}) } {\vert \mathbf{s}_i - \mathbf{r} + \epsilon \vert^3} \times {\bf d}\mathbf{r} \]
\pagebreak

\[ \mathbf{s}_{i'}=\frac{1}{2}(\mathbf{s}_i+\mathbf{s}_{i+1})+\left( \sqrt{R^2_{i'} -\frac{1}{4}\ell_{i+1}^2}-R_{i'} \right)\frac{\mathbf{s}_{i'}''}{|\mathbf{s}_{i'}''|},\]
\pagebreak

$R_{i'}=|\mathbf{s}_{i'}''|^{-1}$
\pagebreak

$ \mathbf{s}_{i'} $
\pagebreak

\[\mathbf{J} \times \mathbf{B}=(\nabla \times \mathbf{B}) \times \mathbf{B} =B^2 d\hat{\mathbf{B}}/ds\]
\pagebreak

\[B(\mathbf{s}_i)=\sum_{j=i-2}^{i+2}B_j\exp{-(\mathbf{s}_i-\mathbf{s}_j)^2/ 4\nu \Delta t}>\]
\pagebreak

\[B(\mathbf{s}_i,t+\Delta t)=\sum_{j=i-2}^{i+2}B_j\exp(-(\mathbf{s}_i -\mathbf{s}_j)^2/4\nu \Delta t)\]
\pagebreak

\[B(\mathbf{s}_i,t+\Delta t)=\sum_{j=i-2}^{i+2}B_j\exp(-(\mathbf{s}_i -\mathbf{s}_j)^2/4\nu \Delta t)\frac{1}{2\sqrt{\pi\nu\Delta t/\ell_j^2}}\]
\pagebreak

\[B(\mathbf{s}_i,t+\Delta t)=\sum_{j=i-2}^{i+2}\exp(-(\mathbf{s}_i -\mathbf{s}_j)^2/4\nu \Delta t)\frac{B_j}{2\sqrt{\pi\nu\Delta t/\ell_j^2}}\]
\pagebreak

\[ \frac{d \mathbf{s}_i}{d \xi}=\frac{\mathbf{s}_{i+1}-\mathbf{s}_{i}}{\ell_i} \]
\pagebreak

$|\mathbf{s}''|$
\pagebreak

$ \partial \rho_i / \partial h_i$
\pagebreak

\[ E=\sqrt{\epsilon^2_p+\Delta^2_0} +\mathbf{p} \cdot \mathbf{v}_s \]
\pagebreak

$ \dot{\mathbf{r}},\dot{\mathbf{p}}$
\pagebreak

$\mathbf{r}$
\pagebreak

$\mathbf{p}$
\pagebreak

\[ \dot{\mathbf{r}}=\frac{\epsilon_p}{\sqrt{\epsilon_p^2+\delta_0^2}} +\frac{\mathbf{p}}{m^*}+\mathbf{u}_s(\mathbf{r},t)\]
\pagebreak

\[ \dot{\mathbf{p}}=-\frac{\partial}{\partial \mathbf{r}} \left [ \mathbf{p} \cdot \mathbf{u}_s(\mathbf{r},t) \right ]\]
\pagebreak

$s\equiv r/h$
\pagebreak

$D=1,\;2,\;{\rm and}\;3\,$
\pagebreak

\begin{eqnarray} W (s) &=& \frac{\sigma_{\!_D}}{h^D} \left\{ \;\; \begin{array}{ll} 1 - \frac{3}{2}s^2 + \frac{3}{4}s^3 \;\;\;\; & \;\;0 \leq s \leq 1\,; \\ \frac{1}{4}(2-s)^3 \;\;\;\; & \;\;1 \leq s \leq 2\,; \\ 0 \;\;\;\; & \;\;s > 2 \,. \end{array} \right . \end{eqnarray}
\pagebreak

$\sigma_{_1}=2/3$
\pagebreak

$\sigma_{_2}=10/7\pi$
\pagebreak

$\sigma_{_3}=1/\pi$
\pagebreak

\begin{eqnarray} \frac{dW}{dr}(s) &=& - \frac{\sigma_{\!_D}}{h^{D+1}} \left\{ \;\; \begin{array}{ll} 3s - \frac{9}{4}s^2 \;\;\;\; & \;\;0 \leq s \leq 1\,; \\ \frac{3}{4}(2-s)^2 \;\;\;\; & \;\;1 \leq s \leq 2\,; \\ 0 \;\;\;\; & \;\;s > 2 \,. \end{array} \right . \end{eqnarray}
\pagebreak

$\Omega$
\pagebreak

\begin{eqnarray} \frac{\partial W}{\partial h}(s) = \frac{\sigma_{\!_D}}{h^{D+1}} \left\{ \;\; \begin{array}{ll} -D + \frac{3}{2}(D + 2)\,s^2 - \frac{3}{4}(D + 3)\,s^3 \;\;\;\; & \;\;0 \leq s \leq 1\,; \\ -2\,D + 3\,(D + 1)\,s - \frac{3}{2}(D + 2)\,s^2 + \frac{1}{4}(D + 3)\,s^3 \;\;\;\; & \;\;1 \leq s \leq 2\,; \\ 0 \;\;\;\; & \;\;s > 2 \,. \end{array} \right . \end{eqnarray}
\pagebreak

\[ h_i = \eta_{_{\rm SPH}} \left( \frac{m_i }{\rho_i} \right)^{\frac{1}{D}}\ \]
\pagebreak

$m_i$
\pagebreak

$i$
\pagebreak

$\rho_i$
\pagebreak

$D$
\pagebreak

$\eta_{_{\rm SPH}}$
\pagebreak

$\bar{N}_{_{\rm NEIB}} \simeq 2\,{\cal R}\,\eta_{_{\rm SPH}} \;,\;\; \pi\,({\cal R}\eta_{_{\rm SPH}})^2 \;,\;\;(4\pi /3)({\cal R}\eta_{_{\rm SPH}})^3\,\,$
\pagebreak

${\cal R}=2$
\pagebreak

$\;\rho_i$
\pagebreak

\[ \rho_i = \sum \limits_{j=1}^{N} m_j W({\bf r}_{ij},h_i), \]
\pagebreak

${\bf r}_{ij} \equiv {\bf r}_i - {\bf r}_j$
\pagebreak

$h_i$
\pagebreak

$h$
\pagebreak

$\rho$
\pagebreak

\begin{eqnarray} \frac{d{\bf v}_i }{dt} &=& - \sum \limits_{j=1}^{N} m_j \left( \frac{P_i}{\Omega_i \rho_i^2} \nabla_i W({\bf r}_{ij} ,h_i) + \frac{P_j}{\Omega_j \rho_j^2} \nabla_i W({\bf r}_{ij} ,h_j) \right) \,, \end{eqnarray}
\pagebreak

$P_i$
\pagebreak

$\nabla_i W$
\pagebreak

\begin{eqnarray} \Omega_i &=& 1 - \frac{\partial h_i }{\partial \rho_i } \sum \limits_{j=1}^{N} m_j \frac{\partial W}{\partial h} ({\bf r}_{ij} , h_i )\,. \end{eqnarray}
\pagebreak

$\Omega_i$
\pagebreak

$\partial h_i / \partial \rho_i$
\pagebreak

$\partial W / \partial h$
\pagebreak

\[ \nabla_i W=\frac{\mathbf{x}_i-\mathbf{x}_j}{{\bf r}_{ij}} \frac{\partial W}{\partial {\bf r}_{ij}} \]
\pagebreak

\end{document}
